wip

Matroid/Connectivity/Multi.lean
@@ -1,4 +1,5 @@
 import Matroid.Connectivity.Local
+import Mathlib.Data.Set.Prod
 
 open Set Function
 
@@ -6,25 +7,82 @@ namespace Matroid
 
 variable {α : Type*} {M : Matroid α} {B B' I I' J J' K X Y : Set α} {ι : Type*}
 
+/-- An auxiliary version of multi-connectivity used in the real definition.
+If the sets are disjoint, then this is equal to `multiConn`, but otherwise it is badly behaved.-/
+noncomputable def multiConnAux (M : Matroid α) (X : ι → Set α) : ℕ∞ :=
+  ⨅ (I : {I : ι → Set α // ∀ i, M.IsBasis' (I i) (X i)}), M.nullity (⋃ i, I.1 i)
+
+lemma multiConnAux_eq_nullity_iUnion (M : Matroid α) {I X : ι → Set α}
+    (hI : ∀ i, M.IsBasis' (I i) (X i)) (hdj : Pairwise (Disjoint on X)) :
+    M.multiConnAux X = M.nullity (⋃ i, I i) := by
+  have aux (J : ι → Set α) (hJ : ∀ i, M.IsBasis' (J i) (X i)) :
+      M.nullity (⋃ i, J i) = M.nullity (⋃ i, I i) := by
+    rw [nullity_iUnion_congr (Y := I)
+      (hdj.mono fun i j ↦ Disjoint.mono (hJ i).subset (hJ j).subset)
+      (hdj.mono fun i j ↦ Disjoint.mono (hI i).subset (hI j).subset)
+      (fun i ↦ by rw [(hI i).indep.nullity_eq, (hJ i).indep.nullity_eq])
+      (fun i ↦ by rw [(hI i).closure_eq_closure, (hJ i).closure_eq_closure])]
+  exact ((iInf_le _ ⟨I, hI⟩).trans (by simp)).antisymm <| by simpa using fun i h ↦ (aux i h).symm.le
+
+/-- The local connectivity of an indexed collection `X : ι → Set α` of sets.
+This is defined indirectly using comaps so that it is meaningful even when the `X` are not disjoint.
+If they are disjoint, it is equal to `M.nullity (⋃ i, I i)` for any bases `I i` for the `X i`;
+see `multiConn_eq_nullity_iUnion`.
+If the `X i` are not disjoint, then there is no simple formula in general, but for pairs,
+an expression using cardinality is given in `multiConn_cond`. -/
 noncomputable def multiConn (M : Matroid α) (X : ι → Set α) : ℕ∞ :=
-  ⨅ (I : {I : ι → Set α // ∀ i, M.IsBasis (I i) (X i)}), M.nullity (⋃ i, I.1 i)
+  (M.comap (Prod.fst : α × ι → α)).multiConnAux fun i ↦ ((· , i) '' (X i))
 
-/-- If `I` and `J` are families of pairwise disjoint independent sets such that `I i` and `J i`
-have the same closure for each `i`, then the unions of `I i` and `J i` have the same nullity. -/
-lemma nullity_switch {X Y : ι → Set α} (hXdj : Pairwise (Disjoint on X))
-    (hYdj : Pairwise (Disjoint on Y)) (hcl : ∀ i, M.closure (X i) = M.closure (Y i))
-    (hnull : ∀ i, M.nullity (X i) = M.nullity (Y i)):
-    M.nullity (⋃ i, X i) = M.nullity (⋃ i, Y i) := by
-  wlog hle : M.nullity (⋃ i, X i) < M.nullity (⋃ i, Y i) generalizing X Y with aux
-  · rw [not_lt] at hle
-    obtain he | hlt := hle.eq_or_lt
-    · rw [he]
-    exact Eq.symm <| aux hYdj hXdj (fun i ↦ (hcl i).symm) (fun i ↦ (hnull i).symm) hlt
-  obtain he | ⟨⟨s⟩⟩ := isEmpty_or_nonempty ι
-  · simp
+lemma multiConn_eq_nullity_iUnion (M : Matroid α) (X I : ι → Set α) (hdj : Pairwise (Disjoint on X))
+    (hIX : ∀ i, M.IsBasis' (I i) (X i)) : M.multiConn X = M.nullity (⋃ i, I i) := by
+  have hinj : InjOn Prod.fst (⋃ i, (·, i) '' I i) := by
+    rintro ⟨x, i⟩ hx ⟨y, j⟩ hy (rfl : x = y)
+    exact Prod.mk_inj.2 ⟨rfl, hdj.eq <| not_disjoint_iff.2
+      ⟨x, (hIX i).subset (by simpa using hx), (hIX j).subset (by simpa using hy)⟩⟩
+  have aux {i : ι} {Y : Set α} : Prod.fst '' ((· , i) '' Y) = Y := by simp [Set.ext_iff]
+  have hbas (i : ι) :
+      (M.comap Prod.fst).IsBasis' ((Prod.mk · i) '' (I i)) ((Prod.mk · i) '' (X i)) := by
+    rw [comap_isBasis'_iff, and_iff_left (image_subset _ (hIX i).subset), aux,
+      aux, and_iff_right (hIX i)]
+    simp [InjOn]
+  rw [multiConn, multiConnAux_eq_nullity_iUnion _ hbas, nullity_comap _ _ hinj, image_iUnion]
+  · simp [aux]
+  simp +contextual [Pairwise, Function.onFun, disjoint_right]
 
-  -- obtain ⟨I, hI⟩
-
-lemma multiConn_eq_of_forall_isBasis {X I : ι → Set α} (hdj : Pairwise (Disjoint on X))
-    (hbas : ∀ i, M.IsBasis (I i) (X i)) : M.multiConn X = M.nullity (⋃ i, I i) := by
-  sorry
+/-- The local connectivity of a pair of sets `X,Y` is the nullity of `I ∪ J` plus the
+cardinality of `I ∩ J`, for any respective bases `I` and `J` for `X` and `Y`. -/
+lemma multiConn_cond (M : Matroid α) (hIX : M.IsBasis' I X) (hJY : M.IsBasis' J Y) :
+    M.multiConn (fun b ↦ bif b then X else Y) = M.nullity (I ∪ J) + (I ∩ J).encard := by
+  have aux_dj (A B : Set α) : Disjoint
+    ((·, true) '' A) ((·, false) '' B) := by simp [disjoint_left]
+  have aux {i : Bool} {Y : Set α}  : Prod.fst '' ((· , i) '' Y) = Y := by simp [Set.ext_iff]
+  have hb (b : Bool) : (M.comap Prod.fst).IsBasis' ((· , b) '' (bif b then I else J))
+      ((· , b) '' (bif b then X else Y)) := by
+    refine comap_isBasis'_iff.2 ⟨?_, by simp [InjOn], image_subset _ ?_ ⟩
+    · obtain rfl | rfl := b
+      · convert hJY <;> simp [Set.ext_iff]
+      convert hIX <;> simp [Set.ext_iff]
+    obtain rfl | rfl := b
+    · exact hJY.subset
+    exact hIX.subset
+  have hi : (M.comap Prod.fst).Indep ((fun x ↦ (x, true)) '' I) := by simp [aux, hIX.indep, InjOn]
+  have hrw : I ∪ J = Prod.fst '' ((fun x ↦ (x, true)) '' I ∪ (fun x ↦ (x, false)) '' (J \ I)) := by
+    suffices ∀ x, x ∈ I ∨ x ∈ J ↔ x ∈ J ∧ x ∉ I ∨ x ∈ I by simpa [Set.ext_iff]
+    tauto
+  rw [multiConn, multiConnAux_eq_nullity_iUnion _ hb]
+  · simp only [iUnion_bool, cond_true, cond_false]
+    rw [← hi.nullity_project_of_disjoint (aux_dj ..),
+      nullity_eq_nullity_add_encard_diff (X := (·, false) '' (J \ I))
+        (image_subset _ (diff_subset)),
+      hi.nullity_project_of_disjoint (aux_dj ..),
+      nullity_comap, ← image_diff (by simp [Injective]), ← hrw,
+      (Prod.mk_left_injective _).encard_image]
+    · simp [inter_comm]
+    · suffices ∀ a, (a ∈ J → a ∉ I → ∀ b ∈ I, ¬a = b) ∧ (a ∈ I → ∀ b ∈ J, b ∉ I → ¬a = b)
+        by simpa [InjOn]
+      aesop
+    · simp only [project_closure, comap_closure_eq, image_subset_iff]
+      rw [← union_comm, ← hrw]
+      simp only [subset_def, mem_preimage]
+      exact fun x hx ↦ M.subset_closure_of_subset' subset_union_right hJY.indep.subset_ground hx
+  simp [Pairwise, pairwise_on_bool, Function.onFun, aux_dj, (aux_dj X Y).symm]
