Matroid/Constructions/QuotientExtension.lean
@@ -1,6 +1,7 @@
 import Matroid.Rank.Skew
 import Matroid.Order.Quotient
 import Matroid.Extension
+import Matroid.ForMathlib.Data.Set.Finite
 
 open Set BigOperators Set.Notation Function
 
@@ -11,6 +12,7 @@ variable {α : Type*} {ι : Type*} {η : Type*} {A : Set η} {M N : Matroid α}
 
 /-- If `N` is a finitary quotient of `M`, then the collection of all flats `F` of `M`
 for which `M.project F = N.project F` is a modular cut. -/
+@[simps!]
 def Quotient.modularCut [N.Finitary] (h : N ≤q M) : M.ModularCut :=
     ModularCut.ofForallIsModularPairChainInter
     (M := M)
@@ -43,9 +45,34 @@ def Quotient.modularCut [N.Finitary] (h : N ≤q M) : M.ModularCut :=
     (h_chain := by
       refine fun Fs hFs hCne hmod hchain ↦ ⟨?_, ?_⟩
       · exact IsFlat.sInter hCne fun F hF ↦ (hFs hF).1
+      simp only [subset_def, mem_setOf_eq] at hFs
       obtain ⟨B, hB, hBmut⟩ := hmod.exists_isMutualBasis_isBase
+      simp only [isMutualBasis_iff, Subtype.forall] at hBmut
       refine Eq.symm <| (h.project_quotient_project _).eq_of_closure_indep (X := B \ ⋂₀ Fs) ?_ ?_
       · simp [hB.spanning.closure_eq_of_superset subset_union_left]
-      sorry
+      rw [indep_iff_forall_subset_not_isCircuit', project_ground, h.ground_eq,
+        and_iff_left (diff_subset.trans hB.subset_ground)]
+      intro C hCss hC
+      have aux (e) (he : e ∈ C) : ∃ F ∈ Fs, e ∉ F := by simpa using (hCss he).2
+      choose! F' hF' using aux
+      replace hchain : IsChain (fun a b ↦ b ≤ a) Fs := hchain.symm
+      have hss' : F' '' C ⊆ Fs := by
+        rw [image_subset_iff, subset_def]
+        exact fun e heC ↦ (hF' e heC).1
+      obtain ⟨F₀, hF₀, hF₀le : ∀ F ∈ F' '' C, F₀ ⊆ F⟩ :=
+        hchain.directedOn.exists_forall_le hCne hss' (hC.finite.image F')
+      have hCi : (N.project F₀).Indep C := by
+        rw [← (hFs _ hF₀).2, (hBmut.2 F₀ hF₀).project_eq_project, project_indep_iff,
+          (hBmut.1.inter_left F₀).contract_indep_iff, inter_comm, disjoint_left]
+        refine ⟨?_, hBmut.1.subset (union_subset (hCss.trans diff_subset) inter_subset_left)⟩
+        rintro e heC ⟨heB, heF₀⟩
+        exact (hF' e heC).2 <| hF₀le (F' e) (mem_image_of_mem _ heC) heF₀
+      refine hC.not_indep (hCi.of_project_subset (sInter_subset_of_mem hF₀)))
 
-    )
+lemma Quotient.foo [N.Finitary] (h : N ≤q M) : N ≤q (M.projectBy h.modularCut) := by
+  set U := h.modularCut with hU
+  refine quotient_of_forall_closure_subset_closure h.ground_eq.symm fun I (hIE : I ⊆ M.E) ↦ ?_
+  wlog hI : (M.projectBy U).Indep I generalizing I with aux
+  · obtain ⟨J, hJ⟩ := (M.projectBy U).exists_isBasis I hIE
+    grw [← hJ.closure_eq_closure, aux _ (hJ.subset.trans hIE) hJ.indep,
+      N.closure_subset_closure hJ.subset]
